proof-libs/fstar/core/Core.Clone.fst
@@ -5,6 +5,7 @@ class t_Clone self = {
 }
 
 (** Everything is clonable *)
+inline_for_extraction
 instance clone_all (t: Type): t_Clone t = {
   f_clone = (fun x -> x);
 }
